Make evaluation of expressions defined on loads that no do touch the memory.
This will be useful for the separation logica assertion. Note that it does
not affect constant expression evaluation in the frontend, as it is first
checked whether the given expression is actually pure (and an expression
containing a load is not).

memory.v
@@ -14,6 +14,8 @@ Section memory_operations.
     Some (to_val Γ w).
   Definition mem_force (Γ : env K) (a : addr K) : mem K → mem K :=
     cmap_alter_ref Γ id (addr_index a) (addr_ref Γ a).
+  Definition mem_forced (Γ : env K) (a : addr K) (m : mem K) : Prop :=
+    mem_force Γ a m = m.
 
   Definition mem_writable (Γ : env K) (a : addr K) (m : mem K) : Prop :=
     ∃ w, m !!{Γ} a = Some w
@@ -498,6 +500,14 @@ Proof.
   destruct m as [m]; simplify_map_equality'; simplify_type_equality.
   by erewrite option_guard_True, to_of_val by eauto.
 Qed.
+Lemma mem_lookup_weaken Γ1 Γ2 Δ m a v τ :
+  ✓ Γ1 → ✓{Γ1,Δ} m → (Γ1,Δ) ⊢ a : TType τ → m !!{Γ1} a = Some v →
+  Γ1 ⊆ Γ2 → m !!{Γ2} a = Some v.
+Proof.
+  unfold lookupE, mem_lookup; rewrite bind_Some; intros ??? (w&?&?) ?.
+  erewrite cmap_lookup_weaken by eauto; simplify_option_equality.
+  by erewrite <-to_val_weaken by eauto.
+Qed.
 
 (** Properties of the [force] function *)
 Lemma mem_force_memenv_of Γ Δ m a :
@@ -533,9 +543,28 @@ Proof.
   unfold valid at 2 3, cmap_valid'; intros.
   erewrite mem_force_memenv_of by eauto; eauto using mem_force_valid.
 Qed.
+Lemma mem_force_weaken Γ1 Γ2 Δ m a τ :
+  ✓ Γ1 → Γ1 ⊆ Γ2 → ✓{Γ1,Δ} m → (Γ1,Δ) ⊢ a : TType τ →
+  mem_force Γ1 a m = mem_force Γ2 a m.
+Proof.
+  unfold mem_force; intros. erewrite addr_ref_weaken by eauto.
+  eauto using cmap_alter_ref_weaken.
+Qed.
+Lemma mem_forced_weaken Γ1 Γ2 Δ m a τ :
+  ✓ Γ1 → Γ1 ⊆ Γ2 → ✓{Γ1,Δ} m → (Γ1,Δ) ⊢ a : TType τ →
+  mem_forced Γ1 a m → mem_forced Γ2 a m.
+Proof. unfold mem_forced; intros. by erewrite <-mem_force_weaken by eauto. Qed.
 Lemma mem_erase_force Γ m a :
   cmap_erase (mem_force Γ a m) = mem_force Γ a (cmap_erase m).
 Proof. apply cmap_erase_alter_ref. Qed.
+Lemma mem_forced_erase Γ a m : mem_forced Γ a (cmap_erase m) ↔ mem_forced Γ a m.
+Proof.
+  unfold mem_forced; split; intros Hm; [|by rewrite <-mem_erase_force, Hm].
+  destruct m as [m]; simplify_equality'; f_equal; apply map_eq; intros o.
+  destruct (decide (o = addr_index a)); simplify_map_equality; auto.
+  apply (f_equal (!! (addr_index a))) in Hm; simplify_map_equality.
+  destruct (m !! _) as [[]|]; simplify_equality'; congruence.
+Qed.
 Lemma mem_lookup_force Γ Δ m a v τ :
   ✓ Γ → ✓{Γ,Δ} m → (Γ,Δ) ⊢ a : TType τ → m !!{Γ} a = Some v → addr_is_obj a →
   mem_force Γ a m !!{Γ} a = Some v.
@@ -568,6 +597,8 @@ Proof.
     !(cmap_alter_ref_le _ _ _ (freeze true <$> addr_ref Γ a2) (addr_ref Γ a2)),
     <-!cmap_alter_ref_compose by eauto using ref_freeze_le_l.
 Qed.
+Lemma mem_force_forced Γ m a : mem_forced Γ a (mem_force Γ a m).
+Proof. unfold mem_forced, mem_force. by rewrite <-cmap_alter_ref_compose. Qed.
 
 (** Properties of the [insert] function *)
 Lemma mem_writable_strict Γ m a : mem_writable Γ a m → addr_strict Γ a.
@@ -704,6 +735,8 @@ Proof.
   unfold insertE, mem_insert, mem_force, cmap_alter.
   by rewrite <-cmap_alter_ref_compose.
 Qed.
+Lemma mem_insert_forced Γ m a v : mem_forced Γ a (<[a:=v]{Γ}>m).
+Proof. symmetry; apply (cmap_alter_ref_compose _ id). Qed.
 Lemma mem_insert_writable Γ Δ m a1 a2 v2 τ2 :
   ✓ Γ → ✓{Γ,Δ} m → a1 = a2 ∨ a1 ⊥{Γ} a2 →
   (Γ,Δ) ⊢ a2 : TType τ2 → mem_writable Γ a2 m → (Γ,Δ) ⊢ v2 : τ2 →
@@ -774,10 +807,9 @@ Proof.
   erewrite ctree_flatten_of_val, zip_with_replicate_l, Forall_fmap by eauto.
   by apply Forall_true.
 Qed.
-Lemma mem_force_singleton Γ Δ a malloc x v τ :
+Lemma mem_singleton_force Γ Δ a malloc x v τ :
   ✓ Γ → (Γ,Δ) ⊢ a : TType τ → addr_strict Γ a →
-  mem_force Γ a (mem_singleton Γ a malloc x v)
-  = mem_singleton Γ a malloc x v.
+  mem_forced Γ a (mem_singleton Γ a malloc x v).
 Proof. apply (cmap_alter_ref_singleton _ Δ id _ _ _ τ). Qed.
 Lemma mem_insert_singleton Γ Δ a malloc x v1 v2 τ :
   ✓ Γ → (Γ,Δ) ⊢ a : TType τ → addr_is_obj a → addr_strict Γ a →
